isabelle/PositiveAccounts.thy
@@ -2,194 +2,195 @@ theory PositiveAccounts
 imports Semantics ValidState
 begin
 
-fun positiveMoneyInAccountOrNoAccount :: "AccountId \<Rightarrow> ((AccountId \<times> Money) list) \<Rightarrow> bool" where
-"positiveMoneyInAccountOrNoAccount accId mlist =
-  (case MList.lookup accId mlist of
+fun positiveMoneyInAccountOrNoAccount :: "AccountId \<Rightarrow> Token \<Rightarrow> Accounts \<Rightarrow> bool" where
+"positiveMoneyInAccountOrNoAccount accId tok mlist =
+  (case MList.lookup (accId, tok) mlist of
      None \<Rightarrow> True
    | Some x \<Rightarrow> x > 0)"
 
 lemma addMoneyToAccountPositve_match :
- "\<forall>x. positiveMoneyInAccountOrNoAccount x accs \<Longrightarrow>
+ "\<forall>x tok. positiveMoneyInAccountOrNoAccount x tok accs \<Longrightarrow>
     money > 0 \<Longrightarrow>
     newBalance > 0 \<Longrightarrow>
-    positiveMoneyInAccountOrNoAccount y (MList.insert y newBalance accs)"
+    positiveMoneyInAccountOrNoAccount y tok2 (MList.insert (y, tok2) newBalance accs)"
   apply simp
   by (simp add: MList.insert_lookup_Some)
 
 lemma addMoneyToAccountPositive_noMatch :
- "\<forall>x. positiveMoneyInAccountOrNoAccount x accs \<Longrightarrow>
+ "\<forall>x tok. positiveMoneyInAccountOrNoAccount x tok accs \<Longrightarrow>
     money > 0 \<Longrightarrow>
-    accId \<noteq> y \<Longrightarrow>
+    (accId, tok) \<noteq> (y, tok2) \<Longrightarrow>
     newBalance > 0 \<Longrightarrow>
-    positiveMoneyInAccountOrNoAccount y (MList.insert accId newBalance accs)"
-  apply simp
-  by (simp add: insert_lookup_different)
+    positiveMoneyInAccountOrNoAccount y tok2 (MList.insert (accId, tok2) newBalance accs)"
+  by (metis addMoneyToAccountPositve_match insert_lookup_different positiveMoneyInAccountOrNoAccount.elims(2) positiveMoneyInAccountOrNoAccount.elims(3))
 
 lemma updateMoneyInAccount_gtZero :
  "0 < newBalance \<Longrightarrow>
-  \<forall>x. positiveMoneyInAccountOrNoAccount x accs \<Longrightarrow>
-  positiveMoneyInAccountOrNoAccount y (updateMoneyInAccount accId newBalance accs)"
+  \<forall>x tok. positiveMoneyInAccountOrNoAccount x tok accs \<Longrightarrow>
+  positiveMoneyInAccountOrNoAccount y tok2 (updateMoneyInAccount accId tok2 newBalance accs)"
   by (metis addMoneyToAccountPositive_noMatch addMoneyToAccountPositve_match not_less updateMoneyInAccount.simps)
-
+  
 lemma addMoneyToAccountPositive :
-  "0 \<le> money \<Longrightarrow> (\<forall>x. positiveMoneyInAccountOrNoAccount x accs)
-  \<Longrightarrow> positiveMoneyInAccountOrNoAccount y (addMoneyToAccount accId money accs)"
+  "(\<forall>x tok. positiveMoneyInAccountOrNoAccount x tok accs)
+  \<Longrightarrow> positiveMoneyInAccountOrNoAccount y tok2 (addMoneyToAccount accId tok3 money accs)"
   apply (simp only:"addMoneyToAccount.simps")
   apply (cases "money \<le> 0")
   apply simp
-  apply (cases "lookup accId accs")
+  apply (metis small_lazy'.cases)
+  apply (cases "lookup (accId, tok3) accs")
   apply simp
-  apply (metis (full_types) MList.insert_lookup_Some insert_lookup_different not_less option.simps(5))
+  apply (metis MList.insert_lookup_Some insert_lookup_different not_le option.simps(5) surj_pair)
   apply simp
-  by (smt MList.insert_lookup_Some insert_lookup_different option.simps(5))
+  by (smt MList.insert_lookup_Some insert_lookup_different option.simps(5) prod_cases3)
 
 lemma giveMoney_gtZero :
-    "\<forall>x. positiveMoneyInAccountOrNoAccount x accs \<Longrightarrow>
-       (eff, newAccs) = giveMoney payee money accs \<Longrightarrow>
-       positiveMoneyInAccountOrNoAccount y newAccs"
-  by (metis addMoneyToAccount.simps addMoneyToAccountPositive giveMoney.elims linear snd_conv)
+    "\<forall>x tok. positiveMoneyInAccountOrNoAccount x tok accs \<Longrightarrow>
+       (eff, newAccs) = giveMoney payee tok2 money accs \<Longrightarrow>
+       positiveMoneyInAccountOrNoAccount y tok3 newAccs"
+  apply (cases payee)
+  apply (simp del:positiveMoneyInAccountOrNoAccount.simps addMoneyToAccount.simps)
+  apply (rule addMoneyToAccountPositive)
+  apply simp
+  apply (simp del:positiveMoneyInAccountOrNoAccount.simps addMoneyToAccount.simps)
+  apply (cases tok3)
+  by blast    
 
-lemma positiveMoneyInAccountOrNoAccount_valid_zero : "valid_map ((accId, money) # rest) \<Longrightarrow> positiveMoneyInAccountOrNoAccount accId rest"
+lemma positiveMoneyInAccountOrNoAccount_valid_zero : "valid_map (((accId, tok), money) # rest) \<Longrightarrow> positiveMoneyInAccountOrNoAccount accId tok rest"
   apply (simp only:positiveMoneyInAccountOrNoAccount.simps findWithDefault.simps)
   by (simp add: MList.delete_lookup_None_aux)
 
 lemma positiveMoneyInAccountOrNoAccount_sublist_gtZero_different :
-  "valid_map ((accId, money) # rest) \<Longrightarrow>
-   0 < money \<Longrightarrow> positiveMoneyInAccountOrNoAccount y ((accId, money) # rest) \<Longrightarrow>
-   accId \<noteq> y \<Longrightarrow> positiveMoneyInAccountOrNoAccount y rest"
+  "valid_map ((accIdTok, money) # rest) \<Longrightarrow>
+   0 < money \<Longrightarrow> positiveMoneyInAccountOrNoAccount y tok ((accIdTok, money) # rest) \<Longrightarrow>
+   accIdTok \<noteq> (y, tok) \<Longrightarrow> positiveMoneyInAccountOrNoAccount y tok rest"
   apply (simp only:positiveMoneyInAccountOrNoAccount.simps findWithDefault.simps)
   by (metis MList.delete.simps(2) MList.different_delete_lookup)
 
 lemma positiveMoneyInAccountOrNoAccount_sublist_gtZero :
-    "valid_map ((accId, money) # rest) \<Longrightarrow>
+    "valid_map ((accIdTok, money) # rest) \<Longrightarrow>
      money > 0 \<Longrightarrow>
-    (\<forall>x. positiveMoneyInAccountOrNoAccount x ((accId, money) # rest)) \<Longrightarrow> positiveMoneyInAccountOrNoAccount y rest"
-  apply (cases "accId = y")
+    (\<forall>x tok. positiveMoneyInAccountOrNoAccount x tok ((accIdTok, money) # rest)) \<Longrightarrow> positiveMoneyInAccountOrNoAccount y tok2 rest"
+  apply (cases "accIdTok = (y, tok2)")
   using positiveMoneyInAccountOrNoAccount_valid_zero apply auto[1]
   using positiveMoneyInAccountOrNoAccount_sublist_gtZero_different by blast
 
 lemma positiveMoneyInAccountOrNoAccount_gtZero_preservation :
-  "valid_map ((accId, money) # rest) \<Longrightarrow>
-   (\<forall>x. positiveMoneyInAccountOrNoAccount x ((accId, money) # rest)) \<Longrightarrow> positiveMoneyInAccountOrNoAccount y rest"
+  "valid_map ((accIdTok, money) # rest) \<Longrightarrow>
+   (\<forall>x tok. positiveMoneyInAccountOrNoAccount x tok ((accIdTok, money) # rest)) \<Longrightarrow> positiveMoneyInAccountOrNoAccount y tok2 rest"
   apply (simp only:positiveMoneyInAccountOrNoAccount.simps findWithDefault.simps)
-  by (metis lookup.simps(2) option.simps(5) positiveMoneyInAccountOrNoAccount.simps positiveMoneyInAccountOrNoAccount_sublist_gtZero)
+  by (metis (no_types, lifting) MList.delete.simps(2) MList.delete_lookup_None MList.sublist_valid delete_step lookup.simps(2) option.simps(4))
 
 lemma reduceOne_gtZero :
   "valid_map accs \<Longrightarrow>
-   \<forall>x. positiveMoneyInAccountOrNoAccount x accs \<Longrightarrow>
+   \<forall>x tok. positiveMoneyInAccountOrNoAccount x tok accs \<Longrightarrow>
    refundOne accs = Some (paym, newAccs) \<Longrightarrow>
-   positiveMoneyInAccountOrNoAccount y newAccs"
+   positiveMoneyInAccountOrNoAccount y tok2 newAccs"
   apply (induction accs rule:"refundOne.induct")
-  subgoal for accId money rest
+  subgoal for accId tok money rest
     apply (cases "money > 0")
-    apply (simp only:refundOne.simps)
-    using positiveMoneyInAccountOrNoAccount_gtZero_preservation apply auto[1]
-    apply (simp only:refundOne.simps if_False)
-    using positiveMoneyInAccountOrNoAccount_gtZero_preservation by auto
+    apply (simp only:refundOne.simps if_True)
+    apply (metis option.inject positiveMoneyInAccountOrNoAccount_gtZero_preservation prod.inject)
+    by (metis MList.sublist_valid positiveMoneyInAccountOrNoAccount_gtZero_preservation refundOne.simps(1))
   by auto
-
-lemma reduceContractStep_gtZero_Refund_aux :
-  "valid_state state \<Longrightarrow>
-   \<forall>x. positiveMoneyInAccountOrNoAccount x (accounts state) \<Longrightarrow>
-   refundOne (accounts state) = Some ((party, money), newAccount) \<Longrightarrow>
-   wa = ReduceNoWarning \<Longrightarrow>
-   eff = ReduceWithPayment (Payment party money) \<Longrightarrow>
-   positiveMoneyInAccountOrNoAccount y newAccount"
-  using reduceOne_gtZero valid_state.elims(2) by blast
 
 lemma reduceContractStep_gtZero_Refund :
   "valid_state state \<Longrightarrow>
-   \<forall>x. positiveMoneyInAccountOrNoAccount x (accounts state) \<Longrightarrow>
-   refundOne (accounts state) = Some ((party, money), newAccount) \<Longrightarrow>
-   Reduced ReduceNoWarning (ReduceWithPayment (Payment party money)) (state\<lparr>accounts := newAccount\<rparr>) Close =
+   \<forall>x tok. positiveMoneyInAccountOrNoAccount x tok (accounts state) \<Longrightarrow>
+   refundOne (accounts state) = Some ((party, tok2, money), newAccount) \<Longrightarrow>
+   Reduced ReduceNoWarning (ReduceWithPayment (Payment party tok2 money)) (state\<lparr>accounts := newAccount\<rparr>) Close =
       Reduced wa eff newState newCont \<Longrightarrow>
-   positiveMoneyInAccountOrNoAccount y (accounts newState)"
-  using reduceContractStep_gtZero_Refund_aux by auto
+   positiveMoneyInAccountOrNoAccount y tok3 (accounts newState)"
+  by (metis (mono_tags) ReduceStepResult.inject State.simps(1) State.surjective State.update_convs(1) reduceOne_gtZero valid_state_valid_accounts)
 
-lemma MList_delete_preserves_gtZero : "valid_map accs \<Longrightarrow> \<forall>x. positiveMoneyInAccountOrNoAccount x accs \<Longrightarrow>
-                                       positiveMoneyInAccountOrNoAccount y (MList.delete accId accs)"
+lemma MList_delete_preserves_gtZero : "valid_map accs \<Longrightarrow> \<forall>x tok. positiveMoneyInAccountOrNoAccount x tok accs \<Longrightarrow>
+                                       positiveMoneyInAccountOrNoAccount y tok2 (MList.delete accIdTok accs)"
   by (metis (full_types) MList.delete_lookup_None MList.different_delete_lookup option.simps(4) positiveMoneyInAccountOrNoAccount.simps)
 
 lemma reduceContractStep_gtZero_Pay_aux :
   "valid_state state \<Longrightarrow>
-   \<forall>x. positiveMoneyInAccountOrNoAccount x (accounts state) \<Longrightarrow>
-   positiveMoneyInAccountOrNoAccount x (updateMoneyInAccount accId amount (accounts state))"
-  using MList_delete_preserves_gtZero updateMoneyInAccount_gtZero by auto
+   \<forall>x tok. positiveMoneyInAccountOrNoAccount x tok (accounts state) \<Longrightarrow>
+   positiveMoneyInAccountOrNoAccount y tok2 (updateMoneyInAccount accId tok3 amount (accounts state))"
+  by (metis MList_delete_preserves_gtZero insert_lookup_different not_le positiveMoneyInAccountOrNoAccount.elims(2) positiveMoneyInAccountOrNoAccount.elims(3) updateMoneyInAccount.simps updateMoneyInAccount_gtZero valid_state_valid_accounts)
 
 lemma reduceContractStep_gtZero_Pay :
   "valid_state state \<Longrightarrow>
-   \<forall>x. positiveMoneyInAccountOrNoAccount x (accounts state) \<Longrightarrow>
-   reduceContractStep env state (Pay accId payee val cont) = Reduced wa eff newState newCont \<Longrightarrow>
-   positiveMoneyInAccountOrNoAccount y (accounts newState)"
+   \<forall>x tok. positiveMoneyInAccountOrNoAccount x tok (accounts state) \<Longrightarrow>
+   reduceContractStep env state (Pay accId payee tok2 val cont) = Reduced wa eff newState newCont \<Longrightarrow>
+   positiveMoneyInAccountOrNoAccount y tok3 (accounts newState)"
   apply (simp only:reduceContractStep.simps)
   apply (cases "evalValue env state val \<le> 0")
   apply simp
-  apply (cases "giveMoney payee (min (moneyInAccount accId (accounts state)) (evalValue env state val))
-                (updateMoneyInAccount accId (moneyInAccount accId (accounts state) - min (moneyInAccount accId (accounts state)) (evalValue env state val))
+  apply (metis prod.collapse)
+  apply (cases "giveMoney payee tok2 (min (moneyInAccount accId tok2 (accounts state)) (evalValue env state val))
+                (updateMoneyInAccount accId tok2
+                  (moneyInAccount accId tok2 (accounts state) - min (moneyInAccount accId tok2 (accounts state)) (evalValue env state val))
                   (accounts state))")
   apply (simp del:positiveMoneyInAccountOrNoAccount.simps valid_state.simps updateMoneyInAccount.simps)
-  by (smt MList_delete_preserves_gtZero ReduceStepResult.inject State.select_convs(1) State.surjective State.update_convs(1) giveMoney_gtZero updateMoneyInAccount.simps updateMoneyInAccount_gtZero valid_state.elims(2))
+  by (metis (no_types, lifting) ReduceStepResult.inject State.simps(1) State.surjective State.update_convs(1) giveMoney_gtZero prod.collapse reduceContractStep_gtZero_Pay_aux)
 
 lemma reduceContractStep_gtZero_Let :
   "valid_state state \<Longrightarrow>
-   \<forall>x. positiveMoneyInAccountOrNoAccount x (accounts state) \<Longrightarrow>
+   \<forall>x tok. positiveMoneyInAccountOrNoAccount x tok (accounts state) \<Longrightarrow>
    reduceContractStep env state (Contract.Let valueId val cont) = Reduced wa eff newState newCont \<Longrightarrow>
-   positiveMoneyInAccountOrNoAccount y (accounts newState)"
+   positiveMoneyInAccountOrNoAccount y tok2 (accounts newState)"
   apply (simp only:reduceContractStep.simps)
   apply (cases "state")
   apply (cases "newState")
   apply (simp del:positiveMoneyInAccountOrNoAccount.simps valid_state.simps)
-  by (metis ReduceStepResult.inject State.ext_inject)
+  by (metis ReduceStepResult.inject State.ext_inject old.prod.exhaust)
 
 theorem reduceContractStep_gtZero :
   "valid_state state \<Longrightarrow>
-   (\<forall>x. positiveMoneyInAccountOrNoAccount x (accounts state)) \<Longrightarrow>
+   (\<forall>x tok. positiveMoneyInAccountOrNoAccount x tok (accounts state)) \<Longrightarrow>
    reduceContractStep env state cont = Reduced wa eff newState newCont \<Longrightarrow>
-   positiveMoneyInAccountOrNoAccount y (accounts newState)"
+   positiveMoneyInAccountOrNoAccount y tok2 (accounts newState)"
   apply (cases cont)
   apply (cases "refundOne (accounts state)")
   apply simp
-  using reduceContractStep_gtZero_Refund apply force
+  apply (metis (mono_tags, lifting) option.simps(5) prod.case_eq_if prod.collapse reduceContractStep.simps(1) reduceContractStep_gtZero_Refund)
   using reduceContractStep_gtZero_Pay apply blast
   apply simp
+  apply (metis prod.collapse)
   apply (smt ReduceStepResult.distinct(1) ReduceStepResult.inject ReduceStepResult.simps(5) case_prod_unfold reduceContractStep.simps(4))
   using reduceContractStep_gtZero_Let by blast
 
 lemma reduceLoop_gtZero : 
   "valid_state state \<Longrightarrow>
-    \<forall>x. positiveMoneyInAccountOrNoAccount x (accounts state) \<Longrightarrow>
+    \<forall>x tok. positiveMoneyInAccountOrNoAccount x tok (accounts state) \<Longrightarrow>
     reductionLoop env state contract warns pays = ContractQuiescent nwa npa newState ncont \<Longrightarrow>
-    positiveMoneyInAccountOrNoAccount y (accounts newState)"
+    positiveMoneyInAccountOrNoAccount y tok2 (accounts newState)"
   apply (induction env state contract warns pays rule: reductionLoop.induct)
   subgoal for env state contract warns pays 
     apply (cases "reduceContractStep env state contract")
     apply (simp only:reductionLoop.simps [of env state contract warns pays])
-    apply (metis (no_types, lifting) ReduceStepResult.simps(8) reduceContractStep_gtZero reductionStep_preserves_valid_state)
+      apply (metis (no_types, lifting) ReduceStepResult.simps(8) reduceContractStep_gtZero reductionStep_preserves_valid_state)
+    apply fastforce
     by simp_all
   done
 
 lemma reduceContractUntilQuiescent_gtZero :
   "valid_state state \<Longrightarrow>
-   (\<forall>x. positiveMoneyInAccountOrNoAccount x (accounts state)) \<Longrightarrow>
+   (\<forall>x tok. positiveMoneyInAccountOrNoAccount x tok (accounts state)) \<Longrightarrow>
    reduceContractUntilQuiescent env state contract = ContractQuiescent nwa npa newState ncont \<Longrightarrow>
-   positiveMoneyInAccountOrNoAccount y (accounts newState)"
+   positiveMoneyInAccountOrNoAccount y tok2 (accounts newState)"
   apply (simp only:reduceContractUntilQuiescent.simps)
   using reduceLoop_gtZero by blast
 
 lemma applyCases_positive : "valid_state state \<Longrightarrow>
-       \<forall>x. positiveMoneyInAccountOrNoAccount x (accounts state) \<Longrightarrow>
+       \<forall>x tok. positiveMoneyInAccountOrNoAccount x tok (accounts state) \<Longrightarrow>
        applyCases env state inp cases = Applied nwa newState ncont \<Longrightarrow>
-       positiveMoneyInAccountOrNoAccount y (accounts newState)"
+       positiveMoneyInAccountOrNoAccount y tok2 (accounts newState)"
   (* Deposit case *)
   apply (induction env state inp cases rule: applyCases.induct)
-  subgoal for env state accId1 party1 money accId2 party2 val cont rest
-    apply (simp only:applyCases.simps(1) [of env state accId1 party1 money accId2 party2 val cont rest])
-    apply (cases "accId1 = accId2 \<and> party1 = party2 \<and> money = ( evalValue env state val)")
+  subgoal for env state accId1 party1 tok1 amount accId2 party2 tok2a val cont rest
+    apply (simp only:applyCases.simps(1) [of env state accId1 party1 tok1 amount accId2 party2 tok2 val cont rest])
+    apply (cases "accId1 = accId2 \<and> party1 = party2 \<and> tok1 = tok2a \<and> amount = evalValue env state val")
     apply (cases " evalValue env state val \<le> 0")
     apply (simp add:Let_def del:valid_state.simps positiveMoneyInAccountOrNoAccount.simps moneyInAccount.simps)
+    apply (metis small_lazy'.cases)
     apply (simp add:Let_def del:valid_state.simps updateMoneyInAccount.simps positiveMoneyInAccountOrNoAccount.simps moneyInAccount.simps)
-    using reduceContractStep_gtZero_Pay_aux apply auto[1]
-  by (simp add:Let_def del:valid_state.simps updateMoneyInAccount.simps positiveMoneyInAccountOrNoAccount.simps moneyInAccount.simps)
+    apply (metis State.simps(1) State.surjective State.update_convs(1) old.prod.exhaust reduceContractStep_gtZero_Pay_aux)
+    by (simp add:Let_def del:valid_state.simps updateMoneyInAccount.simps positiveMoneyInAccountOrNoAccount.simps moneyInAccount.simps)
   (* Choice case *)
   apply (metis ApplyResult.inject State.ext_inject State.simps(7) State.surjective applyCases.simps(2))
   (* Notify case *)
@@ -199,9 +200,9 @@ lemma applyCases_positive : "valid_state state \<Longrightarrow>
 
 lemma applyInput_gtZero :
   "valid_state state \<Longrightarrow>
-   (\<forall>x. positiveMoneyInAccountOrNoAccount x (accounts state)) \<Longrightarrow>
+   (\<forall>x tok. positiveMoneyInAccountOrNoAccount x tok (accounts state)) \<Longrightarrow>
    applyInput env state inp cont = Applied nwa newState ncont \<Longrightarrow>
-   positiveMoneyInAccountOrNoAccount y (accounts newState)"
+   positiveMoneyInAccountOrNoAccount y tok2 (accounts newState)"
   apply (cases cont)
   apply (simp)
   apply (simp)
@@ -212,9 +213,9 @@ lemma applyInput_gtZero :
 
 lemma applyAllLoop_gtZero : 
   "valid_state state \<Longrightarrow>
-   \<forall>x. positiveMoneyInAccountOrNoAccount x (accounts state) \<Longrightarrow>
+   \<forall>x tok. positiveMoneyInAccountOrNoAccount x tok (accounts state) \<Longrightarrow>
    applyAllLoop env state cont inps warns pays = ApplyAllSuccess wa pa newState ncont \<Longrightarrow>
-   positiveMoneyInAccountOrNoAccount y (accounts newState)"
+   positiveMoneyInAccountOrNoAccount y tok2 (accounts newState)"
   apply (induction  env state cont inps warns pays rule: applyAllLoop.induct)
   subgoal for env state contract inputs warnings payments
     apply (cases inputs)
@@ -238,28 +239,26 @@ lemma applyAllLoop_gtZero :
 
 lemma applyAllInputs_gtZero :
   "valid_state state \<Longrightarrow>
-   (\<forall>x. positiveMoneyInAccountOrNoAccount x (accounts state)) \<Longrightarrow>
+   (\<forall>x tok. positiveMoneyInAccountOrNoAccount x tok (accounts state)) \<Longrightarrow>
    applyAllInputs env state cont inps = ApplyAllSuccess wa pa newState ncont \<Longrightarrow>
-   positiveMoneyInAccountOrNoAccount y (accounts newState)"
+   positiveMoneyInAccountOrNoAccount y tok2 (accounts newState)"
   apply (simp only:applyAllInputs.simps)
   using applyAllLoop_gtZero by blast
 
-
 lemma fixInterval_gtZero :
   "valid_state state \<Longrightarrow>
-   (\<forall>x. positiveMoneyInAccountOrNoAccount x (accounts state)) \<Longrightarrow>
+   (\<forall>x tok. positiveMoneyInAccountOrNoAccount x tok (accounts state)) \<Longrightarrow>
    fixInterval inte state = IntervalTrimmed nenv newState \<Longrightarrow>
-   positiveMoneyInAccountOrNoAccount y (accounts newState)"
+   positiveMoneyInAccountOrNoAccount y tok2 (accounts newState)"
   apply (cases  inte)
   apply (simp only:fixInterval.simps)
   by (smt IntervalResult.distinct(1) IntervalResult.inject(1) State.select_convs(1) State.surjective State.update_convs(4))
 
-
 theorem computeTransaction_gtZero :
   "valid_state state \<Longrightarrow>
-   (\<forall>x. positiveMoneyInAccountOrNoAccount x (accounts state)) \<Longrightarrow>
+   (\<forall>x tok. positiveMoneyInAccountOrNoAccount x tok (accounts state)) \<Longrightarrow>
    computeTransaction tx state contract = (TransactionOutput txOut) \<Longrightarrow>
-   positiveMoneyInAccountOrNoAccount y (accounts (txOutState txOut))"
+   positiveMoneyInAccountOrNoAccount y tok2 (accounts (txOutState txOut))"
   apply (simp only:computeTransaction.simps)
   apply (cases "fixInterval (interval tx) state")
   apply (simp only:IntervalResult.case)
@@ -273,11 +272,12 @@ theorem computeTransaction_gtZero :
 
 lemma playTraceAux_gtZero :
   "valid_state (txOutState txIn) \<Longrightarrow>
-   (\<forall>x. positiveMoneyInAccountOrNoAccount x (accounts (txOutState txIn))) \<Longrightarrow>
+   (\<forall>x tok. positiveMoneyInAccountOrNoAccount x tok (accounts (txOutState txIn))) \<Longrightarrow>
    playTraceAux txIn transList = TransactionOutput txOut \<Longrightarrow>
-   positiveMoneyInAccountOrNoAccount y (accounts (txOutState txOut))"
+   positiveMoneyInAccountOrNoAccount y tok2 (accounts (txOutState txOut))"
   apply (induction txIn transList rule:playTraceAux.induct)
   apply simp
+  apply (metis small_lazy'.cases)
   apply (cases txOut)
   subgoal for state cont h t txOutWarnings txOutPayments txOutStatea txOutContract
     apply (simp del:valid_state.simps computeTransaction.simps positiveMoneyInAccountOrNoAccount.simps add:Let_def)
@@ -286,19 +286,19 @@ lemma playTraceAux_gtZero :
     by simp
   done
 
-lemma emptyState_gtZero : "positiveMoneyInAccountOrNoAccount y (accounts (emptyState sl))"
+lemma emptyState_gtZero : "positiveMoneyInAccountOrNoAccount y tok (accounts (emptyState sl))"
   apply simp
   by (simp add: MList.lookup_empty)  
 
 theorem playTrace_gtZero :
   "playTrace sl contract t = TransactionOutput txOut \<Longrightarrow>
-   positiveMoneyInAccountOrNoAccount y (accounts (txOutState txOut))"
+   positiveMoneyInAccountOrNoAccount y tok (accounts (txOutState txOut))"
   by (metis TransactionOutputRecord.select_convs(3) emptyState_gtZero playTrace.simps playTraceAux.simps(1) playTraceAux_gtZero playTrace_preserves_valid_state)
 
 (* Alternative formulation *)
 
-fun allAccountsPositive :: "(AccountId \<times> Money) list \<Rightarrow> bool" where
-"allAccountsPositive accs = foldl (\<lambda> r (_, money) . r \<and> money > 0) True accs"
+fun allAccountsPositive :: "Accounts \<Rightarrow> bool" where
+"allAccountsPositive accs = foldl (\<lambda> r ((_, _), money) . r \<and> money > 0) True accs"
 
 fun allAccountsPositiveState :: "State \<Rightarrow> bool" where
 "allAccountsPositiveState state = allAccountsPositive (accounts state)"
@@ -317,7 +317,8 @@ lemma allAccountsPositiveMeansAllAccountsInTailArePositive_aux :
  "(allAccountsPositive ((a, b) # accs) \<Longrightarrow> allAccountsPositive accs) \<Longrightarrow> allAccountsPositive ((a, b) # aa # accs) \<Longrightarrow> allAccountsPositive (aa # accs)"
   apply simp
   apply (cases "(case aa of (u, x) \<Rightarrow> 0 < x)")
-  by simp_all
+  apply (simp add: case_prod_beta')
+  by (simp add: case_prod_beta')
 
 lemma allAccountsPositiveMeansAllAccountsInTailArePositive :
  "allAccountsPositive ((a, b) # accs) \<Longrightarrow> allAccountsPositive accs"
@@ -326,22 +327,22 @@ lemma allAccountsPositiveMeansAllAccountsInTailArePositive :
   using allAccountsPositiveMeansAllAccountsInTailArePositive_aux by blast
 
 lemma allAccountsPositiveImpliesPositiveMoneyInAccountOrNoAccount_aux :
-  "(\<And>accId. allAccountsPositive accs \<Longrightarrow> positiveMoneyInAccountOrNoAccount accId accs) \<Longrightarrow>
-   allAccountsPositive ((a, b) # accs) \<Longrightarrow> positiveMoneyInAccountOrNoAccount accId ((a, b) # accs)"
+  "(\<And>accId tok. allAccountsPositive accs \<Longrightarrow> positiveMoneyInAccountOrNoAccount accId tok accs) \<Longrightarrow>
+   allAccountsPositive ((a, b) # accs) \<Longrightarrow> positiveMoneyInAccountOrNoAccount accId2 tok2 ((a, b) # accs)"
   apply (simp only:positiveMoneyInAccountOrNoAccount.simps)
-  apply (cases "accId = a")
+  apply (cases "(accId2, tok2) = a")
   apply (simp del:valid_map.simps)
   apply (rule allAccountsPositiveMeansFirstIsPositive)
   apply simp
   apply (simp only:lookup.simps if_False)
-  apply (cases "a < accId")
+  apply (cases "a < (accId2, tok2)")
   apply (simp only:if_True)
   using allAccountsPositiveMeansAllAccountsInTailArePositive apply blast
   by simp
 
 lemma allAccountsPositiveImpliesPositiveMoneyInAccountOrNoAccount :
-  "allAccountsPositive accs \<Longrightarrow> positiveMoneyInAccountOrNoAccount accId accs"
-  apply (induction accs arbitrary: accId)
+  "allAccountsPositive accs \<Longrightarrow> positiveMoneyInAccountOrNoAccount accId tok accs"
+  apply (induction accs arbitrary: accId tok)
   apply simp
   using allAccountsPositiveImpliesPositiveMoneyInAccountOrNoAccount_aux by auto
 
@@ -350,26 +351,26 @@ lemma positiveMoneyInAccountOrNoAccountImpliesAllAccountsPositive_aux :
   by simp
 
 lemma positiveMoneyInAccountOrNoAccountImpliesAllAccountsPositive_aux2 :
-  "(valid_map accs \<Longrightarrow> \<forall>accId. positiveMoneyInAccountOrNoAccount accId accs \<Longrightarrow> allAccountsPositive accs) \<Longrightarrow>
-   valid_map ((a, b) # accs) \<Longrightarrow> \<forall>accId. positiveMoneyInAccountOrNoAccount accId ((a, b) # accs) \<Longrightarrow> allAccountsPositive ((a, b) # accs)"
+  "(valid_map accs \<Longrightarrow> \<forall>accId tok. positiveMoneyInAccountOrNoAccount accId tok accs \<Longrightarrow> allAccountsPositive accs) \<Longrightarrow>
+   valid_map ((a, b) # accs) \<Longrightarrow> \<forall>accId tok. positiveMoneyInAccountOrNoAccount accId tok ((a, b) # accs) \<Longrightarrow> allAccountsPositive ((a, b) # accs)"
   apply (cases "0 \<ge> b")
   apply (simp del:foldl_Cons valid_map.simps)
-  apply (smt option.simps(5))
+  apply (smt old.prod.exhaust option.simps(5))
   apply (simp only:positiveMoneyInAccountOrNoAccount.simps)
   apply (rule positiveMoneyInAccountOrNoAccountImpliesAllAccountsPositive_aux)
   apply linarith
-  using positiveMoneyInAccountOrNoAccount_gtZero_preservation by auto
+  by (meson MList.sublist_valid positiveMoneyInAccountOrNoAccount.simps positiveMoneyInAccountOrNoAccount_gtZero_preservation)
 
 lemma positiveMoneyInAccountOrNoAccountImpliesAllAccountsPositive :
-  "valid_map accs \<Longrightarrow> (\<forall> accId. positiveMoneyInAccountOrNoAccount accId accs) \<Longrightarrow> allAccountsPositive accs"
+  "valid_map accs \<Longrightarrow> (\<forall> accId tok. positiveMoneyInAccountOrNoAccount accId tok accs) \<Longrightarrow> allAccountsPositive accs"
   apply (induction accs)
   apply simp
   using positiveMoneyInAccountOrNoAccountImpliesAllAccountsPositive_aux2 by auto
 
 theorem accountsArePositive :
-  "valid_state state \<Longrightarrow> (\<forall>x. positiveMoneyInAccountOrNoAccount x (accounts state)) \<Longrightarrow>
+  "valid_state state \<Longrightarrow> (\<forall>x tok. positiveMoneyInAccountOrNoAccount x tok (accounts state)) \<Longrightarrow>
   computeTransaction txIn state cont = TransactionOutput txOut \<Longrightarrow>
-  positiveMoneyInAccountOrNoAccount y (accounts (txOutState txOut))"
+  positiveMoneyInAccountOrNoAccount y tok2 (accounts (txOutState txOut))"
   using computeTransaction_gtZero by blast
 
 theorem accountsArePositive2 :
@@ -394,7 +395,7 @@ fun validAndPositive_state :: "State \<Rightarrow> bool" where
 lemma validAndPositiveImpliesValid : "validAndPositive_state state \<Longrightarrow> valid_state state"
   by simp
 
-lemma validAndPositiveImpliesPositive : "validAndPositive_state state \<Longrightarrow> (\<forall> x. positiveMoneyInAccountOrNoAccount x (accounts state))"
+lemma validAndPositiveImpliesPositive : "validAndPositive_state state \<Longrightarrow> (\<forall> x tok. positiveMoneyInAccountOrNoAccount x tok (accounts state))"
   using allAccountsPositiveImpliesPositiveMoneyInAccountOrNoAccount by auto
 
 lemma reduceContractStep_preserves_validAndPositive_state :
